Add lemma chain_imp_fun

spec/Primitives.ec
@@ -1,18 +1,20 @@
 require import AllCore List RealExp IntDiv.
-require (*  *)  Subtype.
-
+require (*  *) Subtype. 
 from Jasmin require import JModel.
 
-require import Notation Address Parameters.
+require import Notation Address.
+require import Array8.
 
-pragma Goals : printall.
+type adrs = W32.t Array8.t.
 
 op n : { int | 0 <= n } as ge0_n.
-op len1 : int = ceil (8%r + n%r / log2 w%r).
-op len2 : int = floor (log2 (len1 * (w-1))%r / log2 w%r) + 1.
+
+op len1 : int = ceil (8%r * n%r / log2 w%r).
+op len2 : int = floor (log2 (len1 * (w - 1))%r / log2 w%r) + 1.
 op len : int = len1 + len2.
 
-lemma ge0_len : 0 <= len by admit. (* or lemma? *)
+(* replaced lemma with axiom *)
+axiom ge0_len : 0 <= len.
 
 clone import Subtype as NBytes with 
    type T = byte list,
@@ -27,49 +29,70 @@ type seed = nbytes.
 op prf : seed -> adrs -> key.
 op f : key -> nbytes -> nbytes.
 
-op nbytexor(a b : nbytes) = 
+op nbytexor(a b : nbytes) : nbytes = 
     map (fun (ab : byte * byte) => ab.`1 `^` ab.`2) (zip a b).
 
 module Chain = {
   proc chain(X : nbytes, i s : int, _seed : seed, address : adrs) : nbytes = {
     var t : nbytes <- X;
-    var _key : key; 
+    var _key : key;
     var chain_count : int <- 0;
     var bitmask : nbytes;
 
+    (* case i + s <= w-1 is precondition *)
     while (chain_count < s) {
-      address <- set_hash_addr address (i + chain_count);
-      address <- set_key_and_mask address 0;
-      _key <- prf _seed address;
-      address <- set_key_and_mask address 1;
-      bitmask <- prf _seed address;
+     address <- set_hash_addr address (i + chain_count);
+     address <- set_key_and_mask address 0;
+     _key <- prf _seed  address;
+     address <- set_key_and_mask address 1;
+     bitmask <- prf _seed address;
 
-      t <- f _key (nbytexor t bitmask);
-      chain_count <- chain_count + 1;
+     t <- f _key (nbytexor t bitmask);
+     chain_count <- chain_count + 1;       
     }
     return t;
   }
 }.
 
-op chain_pre (X : nbytes, i s : int, _seed : seed, address : adrs) = 
-  0 <= s <= w - 1.
+pred chain_pre(X : nbytes, i s : int, _seed : seed, address : adrs) = 
+    0 <= s <= w-1.
 
-op chain (X : nbytes, i s : int, _seed : seed, address : adrs) : nbytes.
+op chain(X : nbytes, i s : int, _seed : seed, address : adrs) : nbytes.
 
 (* Definition of the chain operator for s = 0 *)
-axiom chain0 (X : nbytes, i s : int,  _seed : seed, address) : 
-  s = 0 => chain X i s _seed address = X.
+axiom chain0 (X : nbytes, i s : int, _seed : nbytes, address : adrs) : 
+    s = 0 => chain X i s _seed address = X.
 
-axiom chainS (X : nbytes, i s : int, _seed : seed, address : adrs) :
-  0 < s => chain X i s _seed address = 
-    let t = chain X i (s - 1) _seed address in
-    let address = set_hash_addr address (i + s - 1) in
-    let address = set_key_and_mask address 0 in
-    let _key = prf _seed address in
-    let address = set_key_and_mask address 1 in
-    let bitmask = prf _seed address in
-    let t = f _key (nbytexor t bitmask) in
-    t.
+axiom chainS (X : nbytes, i s : int, _seed : nbytes, address : adrs) :
+    0 < s => chain X i s _seed address =
+      let t = chain X i (s - 1) _seed address in 
+      let address = set_hash_addr address (i + s - 1) in
+      let address = set_key_and_mask address 0 in
+      let _key = prf _seed  address in
+      let address = set_key_and_mask address 1 in
+      let bitmask = prf _seed address in
+      let t = f _key (nbytexor t bitmask) in
+          t.
 
-lemma chain_ll : islossless Chain.chain.
-    by proc; while (true) (s - chain_count); by auto => /#.
+lemma chain_ll : islossless Chain.chain
+  by proc; while (true) (s - chain_count); by auto => /#.
+
+lemma chain_imp_fun (_X : nbytes, _i _s : int, __seed : nbytes, _address : adrs) : 
+  chain_pre _X _i _s __seed _address =>
+  hoare [ Chain.chain : 
+          arg = (_X, _i, _s, __seed, _address) ==>
+             res = chain _X _i _s __seed _address].
+proof. 
+move => pre_cond.
+proc => /=.
+while(_X = X /\ _i = i /\ _s = s /\ __seed = _seed /\ 
+      (forall (k : int), 0 <= k < 6 => _address.[k] = address.[k]) /\ 
+      t = chain _X _i chain_count _seed _address /\
+      0 <= chain_count <= s); last by auto; smt(chain0).
+auto => /> &hr *.
+do split; move => *; 1,3,4: by smt(Array8.set_eqiE Array8.set_neqiE).
+by rewrite (chainS _ _ (chain_count{hr} + 1) _ _) 1:/# /=;
+   congr; congr => /=; [ | congr];
+   apply tP => i  ib;
+   case (i <> 7); smt(Array8.set_eqiE Array8.set_neqiE).
+qed.
